Make solve_cap_pure more robust and document it
In particular, move the notions that can be used in lemma statements
from classes to cap_pure hints, to avoid any unwanted typeclass
resolution.

theories/classes.v
@@ -2,7 +2,11 @@ From Coq Require Import ZArith.
 From stdpp Require Import base option.
 From cap_machine Require Import machine_base machine_parameters addr_reg.
 
-(* Helpers *)
+(* Helper classes. These are used to support proofsearch for automation (of in
+   particular the [solve_cap_pure] tactic). They are not intended to be used
+   directly in program specifications or manual proof scripts. *)
+
+(* Reduction helpers *)
 
 Class SimplTC {A} (x x': A) :=
   MkSimplTc: x = x'.
@@ -10,22 +14,7 @@ Class SimplTC {A} (x x': A) :=
 Class CbvTC {A} (x x': A) :=
   MkCbvTc: x = x'.
 
-(* Address regions *)
-(* XXX Should these be moved to the cap_pure hintsdb? *)
-
-Class ContiguousRegion (a: Addr) (z: Z): Prop :=
-  MkContiguousRegion: is_Some (a + z)%a.
-Hint Mode ContiguousRegion + - : typeclass_instances.
-
-Class SubBounds (b e: Addr) (b' e': Addr) :=
-  MkSubBounds: (b <= b')%a ∧ (b' <= e')%a ∧ (e' <= e)%a.
-Hint Mode SubBounds + + - - : typeclass_instances.
-
-Class InBounds (b e: Addr) (a: Addr) :=
-  MkInBounds: (b <= a)%a ∧ (a < e)%a.
-Hint Mode InBounds + + + : typeclass_instances.
-
-(* Address manipulation *)
+(* Address arithmetic *)
 
 Class AddrOffsetLt z z' := MkAddrOffsetLt: (z < z')%Z.
 Hint Mode AddrOffsetLt + + : typeclass_instances.
@@ -50,12 +39,6 @@ Class AddrEq (a b: Addr) (res: bool) :=
 Hint Mode AddrEq + + - : typeclass_instances.
 
 (* Other *)
-
-Class ExecPCPerm p :=
-  MkExecPcPerm: p = RX ∨ p = RWX.
-Hint Mode ExecPCPerm + : typeclass_instances.
-
-Existing Class PermFlows.
 
 Class DecodeInstr `{MachineParameters} (w: Word) (i: instr) :=
   MkDecodeInstr: decodeInstrW w = i.
